secp256k1: use precomputed table with w = 5 for GLV

code/k256/Hacl.Impl.K256.GLV.fst
@@ -28,34 +28,49 @@ open Hacl.Impl.K256.Point
 
 open Hacl.Impl.K256.GLV.Constants
 include Hacl.Impl.K256.Group
+include Hacl.K256.PrecompTable
 
 #set-options "--z3rlimit 50 --fuel 0 --ifuel 0"
 
-(**
- Fast computation of [scalar]Q in projective coordinates
-*)
+let _: squash(pow2 5 = 32) =
+  assert_norm (pow2 5 = 32)
+
+let _: squash(pow2 128 < S.q) =
+  assert_norm (pow2 128 < S.q)
+
+
+inline_for_extraction noextract
+let table_inv_w5 : BE.table_inv_t U64 15ul 32ul =
+  [@inline_let] let len = 15ul in
+  [@inline_let] let ctx_len = 0ul in
+  [@inline_let] let k = mk_k256_concrete_ops in
+  [@inline_let] let l = 5ul in
+  [@inline_let] let table_len = 32ul in
+  BE.table_inv_precomp len ctx_len k l table_len
+
 
 inline_for_extraction noextract
 let table_neg_inv_precomp
-  (q:LSeq.lseq uint64 15) (is_negate:bool) : BE.table_inv_t U64 15ul 16ul =
+  (q:LSeq.lseq uint64 15) (is_negate:bool) : BE.table_inv_t U64 15ul 32ul =
   fun a table ->
     point_eval_lseq a == SG.point_negate_cond (point_eval_lseq q) is_negate /\
-    (forall (j:nat{j < 16}).
-      PT.precomp_table_inv 15ul 0ul mk_k256_concrete_ops q 16ul table j)
+    (forall (j:nat{j < 32}).
+      PT.precomp_table_inv 15ul 0ul mk_k256_concrete_ops q 32ul table j)
+
 
 // This function returns [r_small]Q or [r_small](-Q)
 // using a precomputed table [0; Q; 2Q; ...; 15Q]
 inline_for_extraction noextract
 val lprecomp_get_vartime_neg:
     q:Ghost.erased (LSeq.lseq uint64 15){point_inv_lseq q} -> is_negate:bool ->
-  BE.pow_a_to_small_b_st U64 15ul 0ul mk_k256_concrete_ops 4ul 16ul
+  BE.pow_a_to_small_b_st U64 15ul 0ul mk_k256_concrete_ops 5ul 32ul
     (table_neg_inv_precomp q is_negate)
 
 let lprecomp_get_vartime_neg q is_negate ctx lambda_q table r_small res =
   let h0 = ST.get () in
   assert (table_neg_inv_precomp q is_negate lambda_q (as_seq h0 table));
   // table.[r_small] = [r_small]Q
-  BE.lprecomp_get_vartime 15ul 0ul mk_k256_concrete_ops 4ul 16ul ctx q table r_small res;
+  BE.lprecomp_get_vartime 15ul 0ul mk_k256_concrete_ops 5ul 32ul ctx q table r_small res;
   SE.pow_lemma S.mk_k256_concrete_ops (point_eval_lseq q) (v r_small);
   let h1 = ST.get () in
   assert (S.to_aff_point (point_eval h1 res) ==
@@ -77,12 +92,12 @@ let lprecomp_get_vartime_neg q is_negate ctx lambda_q table r_small res =
 
 inline_for_extraction noextract
 let table_lambda_neg_inv_precomp
-  (q:LSeq.lseq uint64 15) (is_negate:bool) : BE.table_inv_t U64 15ul 16ul =
+  (q:LSeq.lseq uint64 15) (is_negate:bool) : BE.table_inv_t U64 15ul 32ul =
   fun a table ->
     point_eval_lseq a ==
       SG.point_negate_cond (SG.point_mul_lambda (point_eval_lseq q)) is_negate /\
-    (forall (j:nat{j < 16}).
-      PT.precomp_table_inv 15ul 0ul mk_k256_concrete_ops q 16ul table j)
+    (forall (j:nat{j < 32}).
+      PT.precomp_table_inv 15ul 0ul mk_k256_concrete_ops q 32ul table j)
 
 
 // This function returns [r_small]([lambda]Q) or [r_small](-[lambda]Q)
@@ -90,14 +105,14 @@ let table_lambda_neg_inv_precomp
 inline_for_extraction noextract
 val lprecomp_get_vartime_lambda_neg:
     q:Ghost.erased (LSeq.lseq uint64 15){point_inv_lseq q} -> is_negate:bool ->
-  BE.pow_a_to_small_b_st U64 15ul 0ul mk_k256_concrete_ops 4ul 16ul
+  BE.pow_a_to_small_b_st U64 15ul 0ul mk_k256_concrete_ops 5ul 32ul
     (table_lambda_neg_inv_precomp q is_negate)
 
 let lprecomp_get_vartime_lambda_neg q is_negate ctx lambda_q table r_small res =
   let h0 = ST.get () in
   assert (table_lambda_neg_inv_precomp q is_negate lambda_q (as_seq h0 table));
   // table.[r_small] = [r_small]Q
-  BE.lprecomp_get_vartime 15ul 0ul mk_k256_concrete_ops 4ul 16ul ctx q table r_small res;
+  BE.lprecomp_get_vartime 15ul 0ul mk_k256_concrete_ops 5ul 32ul ctx q table r_small res;
   SE.pow_lemma S.mk_k256_concrete_ops (point_eval_lseq q) (v r_small);
   let h1 = ST.get () in
   assert (S.to_aff_point (point_eval h1 res) ==
@@ -129,169 +144,9 @@ let lprecomp_get_vartime_lambda_neg q is_negate ctx lambda_q table r_small res =
 //------------------------------
 
 inline_for_extraction noextract
-val point_mul_split_lambda_table:
-  out:point -> r1:qelem -> q1:point -> r2:qelem -> q2:point
-  -> p:point -> is_negate1:bool -> is_negate2:bool -> Stack unit
-  (requires fun h ->
-    live h out /\ live h r1 /\ live h r2 /\
-    live h q1 /\ live h q2 /\ live h p /\
-    eq_or_disjoint q1 q2 /\ disjoint out q1 /\ disjoint out q2 /\
-    disjoint out r1 /\ disjoint out r2 /\ disjoint out p /\
-    point_inv h q1 /\ point_inv h q2 /\ point_inv h p /\
-    point_eval h q1 == SG.point_negate_cond (point_eval h p) is_negate1 /\
-    point_eval h q2 == SG.point_negate_cond (SG.point_mul_lambda (point_eval h p)) is_negate2 /\
-    qas_nat h r1 < S.q /\ qas_nat h r1 < pow2 128 /\
-    qas_nat h r2 < S.q /\ qas_nat h r2 < pow2 128)
-  (ensures  fun h0 _ h1 -> modifies (loc out) h0 h1 /\
-    point_inv h1 out /\
-    refl (as_seq h1 out) ==
-      LE.exp_double_fw S.mk_k256_comm_monoid
-        (refl (as_seq h0 q1)) 128 (qas_nat h0 r1)
-        (refl (as_seq h0 q2)) (qas_nat h0 r2) 4)
-
-let point_mul_split_lambda_table out r1 q1 r2 q2 p is_negate1 is_negate2 =
-  [@inline_let] let len = 15ul in
-  [@inline_let] let ctx_len = 0ul in
-  [@inline_let] let k = mk_k256_concrete_ops in
-  [@inline_let] let l = 4ul in
-  [@inline_let] let table_len = 16ul in
-  [@inline_let] let bLen = 4ul in
-  [@inline_let] let bBits = 128ul in
-
-  let h0 = ST.get () in
-  push_frame ();
-  let table = create (table_len *! len) (u64 0) in
-  PT.lprecomp_table len ctx_len k (null uint64) p table_len table;
-  let h1 = ST.get () in
-  assert (forall (j:nat{j < v table_len}).
-    PT.precomp_table_inv len ctx_len k (as_seq h1 p) table_len (as_seq h1 table) j);
-
-  assert (point_eval_lseq (as_seq h1 q1) ==
-    SG.point_negate_cond (point_eval_lseq (as_seq h1 p)) is_negate1);
-  [@inline_let]
-  let table_inv1 : BE.table_inv_t U64 len table_len =
-    table_neg_inv_precomp (as_seq h0 p) is_negate1 in
-  assert (table_inv1 (as_seq h1 q1) (as_seq h1 table));
-
-  assert (point_eval_lseq (as_seq h1 q2) ==
-    SG.point_negate_cond (SG.point_mul_lambda (point_eval_lseq (as_seq h1 p))) is_negate2);
-  [@inline_let]
-  let table_inv2 : BE.table_inv_t U64 len table_len =
-    table_lambda_neg_inv_precomp (as_seq h0 p) is_negate2 in
-  assert (table_inv2 (as_seq h1 q2) (as_seq h1 table));
-
-  ME.mk_lexp_double_fw_tables len ctx_len k l table_len
-    table_inv1 table_inv2
-    (lprecomp_get_vartime_neg (as_seq h0 p) is_negate1)
-    (lprecomp_get_vartime_lambda_neg (as_seq h0 p) is_negate2)
-    (null uint64) q1 bLen bBits r1 q2 r2 (to_const table) (to_const table) out;
-  pop_frame ()
-
-
-// [scalar]Q = [(r1 + r2 * lambda) % S.q]Q = [r1]Q + [r2]([lambda]Q)
-inline_for_extraction noextract
-val point_mul_split_lambda_vartime: out:point -> scalar:qelem -> q:point -> Stack unit
-  (requires fun h ->
-    live h out /\ live h scalar /\ live h q /\
-    disjoint out q /\ disjoint out scalar /\ disjoint q scalar /\
-    point_inv h q /\ qas_nat h scalar < S.q)
-  (ensures  fun h0 _ h1 -> modifies (loc out) h0 h1 /\
-    point_inv h1 out /\
-    S.to_aff_point (point_eval h1 out) ==
-      S.aff_point_mul (qas_nat h0 scalar) (S.to_aff_point (point_eval h0 q)))
-
-let point_mul_split_lambda_vartime out scalar q =
-  let h0 = ST.get () in
-  push_frame ();
-  let r1 = create_qelem () in
-  let r2 = create_qelem () in
-  let q1 = create_point () in
-  let q2 = create_point () in
-  let is_high1, is_high2 = ecmult_endo_split r1 r2 q1 q2 scalar q in
-  let h1 = ST.get () in
-  assert (modifies (loc r1 |+| loc r2 |+| loc q1 |+| loc q2) h0 h1);
-  point_mul_split_lambda_table out r1 q1 r2 q2 q is_high1 is_high2;
-  let h2 = ST.get () in
-  assert (modifies (loc out) h1 h2);
-  assert (modifies (loc r1 |+| loc r2 |+| loc q1 |+| loc q2 |+| loc out) h0 h2);
-  pop_frame ();
-  let h3 = ST.get () in
-  assert (modifies (loc out) h0 h3);
-  assert (S.to_aff_point (point_eval h3 out) ==
-    SGL.aff_proj_point_mul_split_lambda (qas_nat h0 scalar) (point_eval h0 q));
-  SGL.lemma_aff_proj_point_mul_split_lambda (qas_nat h0 scalar) (point_eval h0 q)
-
-
-// TODO: precompute a table [0; G; 2G; ..; 15G]?
-val point_mul_g_split_lambda_vartime: out:point -> scalar:qelem -> Stack unit
-  (requires fun h ->
-    live h out /\ live h scalar /\ disjoint out scalar /\
-    qas_nat h scalar < S.q)
-  (ensures  fun h0 _ h1 -> modifies (loc out) h0 h1 /\
-    point_inv h1 out /\
-    S.to_aff_point (point_eval h1 out) ==
-      S.aff_point_mul (qas_nat h0 scalar) (S.g_x, S.g_y))
-
-[@CInline]
-let point_mul_g_split_lambda_vartime out scalar =
-  SL.lemma_proj_aff_id (S.g_x, S.g_y);
-  push_frame ();
-  let g = create 15ul (u64 0) in
-  make_g g;
-  point_mul_split_lambda_vartime out scalar g;
-  pop_frame ()
-
-
-(**
- Fast computation of [scalar1]Q1 + [scalar2]Q2 in projective coordinates
-*)
-
-inline_for_extraction noextract
-val mk_two_tables:
-    table1:lbuffer uint64 (16ul *! 15ul)
-  -> table2:lbuffer uint64 (16ul *! 15ul)
-  -> p1:point -> p2:point ->
-  Stack unit
-  (requires fun h ->
-    live h table1 /\ live h table2 /\ live h p1 /\ live h p2 /\
-    disjoint table1 table2 /\ disjoint table1 p1 /\ disjoint table1 p2 /\
-    disjoint table2 p1 /\ disjoint table2 p2 /\
-    point_inv h p1 /\ point_inv h p2)
-  (ensures fun h0 _ h1 -> modifies (loc table1 |+| loc table2) h0 h1 /\
-   (let len = 15ul in
-    let ctx_len = 0ul in
-    let k = mk_k256_concrete_ops in
-    let l = 4ul in
-    let table_len = 16ul in
-    BE.table_inv_precomp len ctx_len k l table_len (as_seq h0 p1) (as_seq h1 table1) /\
-    BE.table_inv_precomp len ctx_len k l table_len (as_seq h0 p2) (as_seq h1 table2)))
-
-let mk_two_tables table1 table2 p1 p2 =
-  [@inline_let] let len = 15ul in
-  [@inline_let] let ctx_len = 0ul in
-  [@inline_let] let k = mk_k256_concrete_ops in
-  [@inline_let] let l = 4ul in
-  [@inline_let] let table_len = 16ul in
-
-  let h0 = ST.get () in
-  PT.lprecomp_table len ctx_len k (null uint64) p1 table_len table1;
-  let h1 = ST.get () in
-  assert (BE.table_inv_precomp len ctx_len k l table_len
-    (as_seq h1 p1) (as_seq h1 table1));
-
-  PT.lprecomp_table len ctx_len k (null uint64) p2 table_len table2;
-  let h2 = ST.get () in
-  assert (BE.table_inv_precomp len ctx_len k l table_len
-    (as_seq h2 p1) (as_seq h2 table1));
-  assert (BE.table_inv_precomp len ctx_len k l table_len
-    (as_seq h2 p2) (as_seq h2 table2))
-
-
-inline_for_extraction noextract
-val point_mul_double_split_lambda_table_noalloc:
+val point_mul_g_double_split_lambda_table_noalloc:
     out:point
-  -> table1:lbuffer uint64 (16ul *! 15ul)
-  -> table2:lbuffer uint64 (16ul *! 15ul)
+  -> table2:lbuffer uint64 (32ul *! 15ul)
   -> r1:qelem -> q1:point
   -> r2:qelem -> q2:point
   -> r3:qelem -> q3:point
@@ -301,20 +156,16 @@ val point_mul_double_split_lambda_table_noalloc:
   -> is_negate3:bool -> is_negate4:bool ->
   Stack unit
   (requires fun h ->
-    live h out /\ live h r1 /\ live h r2 /\ live h r3 /\ live h r4 /\
+    live h out /\ live h table2 /\
+    live h r1 /\ live h r2 /\ live h r3 /\ live h r4 /\
     live h q1 /\ live h q2 /\ live h q3 /\ live h q4 /\
-    live h p1 /\ live h p2 /\ live h table1 /\ live h table2 /\
+    live h p1 /\ live h p2 /\
 
     eq_or_disjoint q1 q2 /\ eq_or_disjoint q1 q3 /\ eq_or_disjoint q1 q4 /\
     eq_or_disjoint q2 q3 /\ eq_or_disjoint q2 q4 /\ eq_or_disjoint q3 q4 /\
     disjoint out q1 /\ disjoint out q2 /\ disjoint out q3 /\ disjoint out q4 /\
     disjoint out r1 /\ disjoint out r2 /\ disjoint out r3 /\ disjoint out r4 /\
-    disjoint out p1  /\ disjoint out p2 /\ disjoint table1 table2 /\
-
-    disjoint table1 out /\ disjoint table1 r1 /\ disjoint table1 r2 /\
-    disjoint table1 r3 /\ disjoint table1 r4 /\  disjoint table1 p1 /\
-    disjoint table1 p2 /\ disjoint table1 q1 /\ disjoint table1 q2 /\
-    disjoint table1 q3 /\ disjoint table1 q4 /\
+    disjoint out p1  /\ disjoint out p2 /\
 
     disjoint table2 out /\ disjoint table2 r1 /\ disjoint table2 r2 /\
     disjoint table2 r3 /\ disjoint table2 r4 /\  disjoint table2 p1 /\
@@ -323,6 +174,7 @@ val point_mul_double_split_lambda_table_noalloc:
 
     point_inv h q1 /\ point_inv h q2 /\ point_inv h q3 /\ point_inv h q4 /\
     point_inv h p1 /\ point_inv h p2 /\
+    point_eval h p1 == S.g /\
     point_eval h q1==SG.point_negate_cond (point_eval h p1) is_negate1 /\
     point_eval h q2==SG.point_negate_cond (SG.point_mul_lambda (point_eval h p1)) is_negate2 /\
     point_eval h q3==SG.point_negate_cond (point_eval h p2) is_negate3 /\
@@ -330,47 +182,47 @@ val point_mul_double_split_lambda_table_noalloc:
     qas_nat h r1 < S.q /\ qas_nat h r1 < pow2 128 /\
     qas_nat h r2 < S.q /\ qas_nat h r2 < pow2 128 /\
     qas_nat h r3 < S.q /\ qas_nat h r3 < pow2 128 /\
-    qas_nat h r4 < S.q /\ qas_nat h r4 < pow2 128)
-  (ensures  fun h0 _ h1 -> modifies (loc out |+| loc table1 |+| loc table2) h0 h1 /\
+    qas_nat h r4 < S.q /\ qas_nat h r4 < pow2 128 /\
+    table_inv_w5 (as_seq h p2) (as_seq h table2))
+  (ensures  fun h0 _ h1 -> modifies (loc out) h0 h1 /\
     point_inv h1 out /\
     refl (as_seq h1 out) ==
       LE.exp_four_fw S.mk_k256_comm_monoid
         (refl (as_seq h0 q1)) 128 (qas_nat h0 r1)
         (refl (as_seq h0 q2)) (qas_nat h0 r2)
         (refl (as_seq h0 q3)) (qas_nat h0 r3)
-        (refl (as_seq h0 q4)) (qas_nat h0 r4) 4)
+        (refl (as_seq h0 q4)) (qas_nat h0 r4) 5)
 
-let point_mul_double_split_lambda_table_noalloc out table1 table2 r1 q1 r2 q2 r3 q3 r4 q4
-  p1 p2 is_negate1 is_negate2 is_negate3 is_negate4 =
+let point_mul_g_double_split_lambda_table_noalloc out table2 r1 q1 r2 q2 r3 q3 r4 q4 p1 p2
+  is_negate1 is_negate2 is_negate3 is_negate4 =
   [@inline_let] let len = 15ul in
   [@inline_let] let ctx_len = 0ul in
   [@inline_let] let k = mk_k256_concrete_ops in
-  [@inline_let] let l = 4ul in
-  [@inline_let] let table_len = 16ul in
+  [@inline_let] let l = 5ul in
+  [@inline_let] let table_len = 32ul in
   [@inline_let] let bLen = 4ul in
   [@inline_let] let bBits = 128ul in
 
   let h0 = ST.get () in
-  mk_two_tables table1 table2 p1 p2;
+  recall_contents precomp_basepoint_table_w5 precomp_basepoint_table_lseq_w5;
   let h1 = ST.get () in
-  assert (forall (j:nat{j < v table_len}).
-    PT.precomp_table_inv len ctx_len k (as_seq h1 p1) table_len (as_seq h1 table1) j);
-  assert (forall (j:nat{j < v table_len}).
-    PT.precomp_table_inv len ctx_len k (as_seq h1 p2) table_len (as_seq h1 table2) j);
+  precomp_basepoint_table_lemma_w5 ();
+  assert (table_inv_w5 (as_seq h1 p1) (as_seq h1 precomp_basepoint_table_w5));
+  assert (table_inv_w5 (as_seq h1 p2) (as_seq h1 table2));
 
   assert (point_eval_lseq (as_seq h1 q1) ==
     SG.point_negate_cond (point_eval_lseq (as_seq h1 p1)) is_negate1);
   [@inline_let]
   let table_inv1 : BE.table_inv_t U64 len table_len =
     table_neg_inv_precomp (as_seq h0 p1) is_negate1 in
-  assert (table_inv1 (as_seq h1 q1) (as_seq h1 table1));
+  assert (table_inv1 (as_seq h1 q1) (as_seq h1 precomp_basepoint_table_w5));
 
   assert (point_eval_lseq (as_seq h1 q2) ==
     SG.point_negate_cond (SG.point_mul_lambda (point_eval_lseq (as_seq h1 p1))) is_negate2);
   [@inline_let]
   let table_inv2 : BE.table_inv_t U64 len table_len =
     table_lambda_neg_inv_precomp (as_seq h0 p1) is_negate2 in
-  assert (table_inv2 (as_seq h1 q2) (as_seq h1 table1));
+  assert (table_inv2 (as_seq h1 q2) (as_seq h1 precomp_basepoint_table_w5));
 
   assert (point_eval_lseq (as_seq h1 q3) ==
     SG.point_negate_cond (point_eval_lseq (as_seq h1 p2)) is_negate3);
@@ -386,8 +238,6 @@ let point_mul_double_split_lambda_table_noalloc out table1 table2 r1 q1 r2 q2 r3
     table_lambda_neg_inv_precomp (as_seq h0 p2) is_negate4 in
   assert (table_inv4 (as_seq h1 q4) (as_seq h1 table2));
 
-  assert (modifies (loc table1 |+| loc table2) h0 h1);
-
   ME.mk_lexp_four_fw_tables len ctx_len k l table_len
     table_inv1 table_inv2 table_inv3 table_inv4
     (lprecomp_get_vartime_neg (as_seq h0 p1) is_negate1)
@@ -395,23 +245,13 @@ let point_mul_double_split_lambda_table_noalloc out table1 table2 r1 q1 r2 q2 r3
     (lprecomp_get_vartime_neg (as_seq h0 p2) is_negate3)
     (lprecomp_get_vartime_lambda_neg (as_seq h0 p2) is_negate4)
     (null uint64) q1 bLen bBits r1 q2 r2 q3 r3 q4 r4
-    (to_const table1) (to_const table1) (to_const table2) (to_const table2) out;
-
-  let h2 = ST.get () in
-  assert (modifies (loc out) h1 h2);
-  assert (point_inv h2 out /\
-    refl (as_seq h2 out) ==
-      LE.exp_four_fw S.mk_k256_comm_monoid
-        (refl (as_seq h0 q1)) 128 (qas_nat h0 r1)
-        (refl (as_seq h0 q2)) (qas_nat h0 r2)
-        (refl (as_seq h0 q3)) (qas_nat h0 r3)
-        (refl (as_seq h0 q4)) (qas_nat h0 r4) 4);
-
-  assert (modifies (loc table1 |+| loc table2 |+| loc out) h0 h2)
+    (to_const precomp_basepoint_table_w5)
+    (to_const precomp_basepoint_table_w5)
+    (to_const table2) (to_const table2) out
 
 
 inline_for_extraction noextract
-val point_mul_double_split_lambda_table:
+val point_mul_g_double_split_lambda_table:
     out:point
   -> r1:qelem -> q1:point
   -> r2:qelem -> q2:point
@@ -431,6 +271,7 @@ val point_mul_double_split_lambda_table:
     disjoint out p1  /\ disjoint out p2 /\
     point_inv h q1 /\ point_inv h q2 /\ point_inv h q3 /\ point_inv h q4 /\
     point_inv h p1 /\ point_inv h p2 /\
+    point_eval h p1 == S.g /\
     point_eval h q1==SG.point_negate_cond (point_eval h p1) is_negate1 /\
     point_eval h q2==SG.point_negate_cond (SG.point_mul_lambda (point_eval h p1)) is_negate2 /\
     point_eval h q3==SG.point_negate_cond (point_eval h p2) is_negate3 /\
@@ -446,28 +287,30 @@ val point_mul_double_split_lambda_table:
         (refl (as_seq h0 q1)) 128 (qas_nat h0 r1)
         (refl (as_seq h0 q2)) (qas_nat h0 r2)
         (refl (as_seq h0 q3)) (qas_nat h0 r3)
-        (refl (as_seq h0 q4)) (qas_nat h0 r4) 4)
+        (refl (as_seq h0 q4)) (qas_nat h0 r4) 5)
 
-let point_mul_double_split_lambda_table out r1 q1 r2 q2 r3 q3 r4 q4
+let point_mul_g_double_split_lambda_table out r1 q1 r2 q2 r3 q3 r4 q4
   p1 p2 is_negate1 is_negate2 is_negate3 is_negate4 =
   [@inline_let] let len = 15ul in
-  [@inline_let] let table_len = 16ul in
+  [@inline_let] let ctx_len = 0ul in
+  [@inline_let] let k = mk_k256_concrete_ops in
+  [@inline_let] let table_len = 32ul in
 
   let h0 = ST.get () in
   push_frame ();
-  let table1 = create (table_len *! len) (u64 0) in
   let table2 = create (table_len *! len) (u64 0) in
-  point_mul_double_split_lambda_table_noalloc out table1 table2 r1 q1 r2 q2 r3 q3 r4 q4
-  p1 p2 is_negate1 is_negate2 is_negate3 is_negate4;
+  PT.lprecomp_table len ctx_len k (null uint64) p2 table_len table2;
+  point_mul_g_double_split_lambda_table_noalloc out table2 r1 q1 r2 q2 r3 q3 r4 q4
+    p1 p2 is_negate1 is_negate2 is_negate3 is_negate4;
   let h1 = ST.get () in
-  assert (modifies (loc out |+| loc table1 |+| loc table2) h0 h1);
+  assert (modifies (loc out |+| loc table2) h0 h1);
   pop_frame ();
   let h2 = ST.get () in
   assert (modifies (loc out) h0 h2)
 
 
 inline_for_extraction noextract
-val point_mul_double_split_lambda_vartime_noalloc_12:
+val point_mul_g_double_split_lambda_vartime_endo_split:
     r1:qelem -> q1:point
   -> r2:qelem -> q2:point
   -> r3:qelem -> q3:point
@@ -528,7 +371,7 @@ val point_mul_double_split_lambda_vartime_noalloc_12:
     is_high3 == S.scalar_is_high r3_s0 /\
     is_high4 == S.scalar_is_high r4_s0))
 
-let point_mul_double_split_lambda_vartime_noalloc_12 r1 q1 r2 q2 r3 q3 r4 q4
+let point_mul_g_double_split_lambda_vartime_endo_split r1 q1 r2 q2 r3 q3 r4 q4
   scalar1 scalar2 p1 p2 =
   let is_high1, is_high2 = ecmult_endo_split r1 r2 q1 q2 scalar1 p1 in
   let is_high3, is_high4 = ecmult_endo_split r3 r4 q3 q4 scalar2 p2 in
@@ -536,7 +379,7 @@ let point_mul_double_split_lambda_vartime_noalloc_12 r1 q1 r2 q2 r3 q3 r4 q4
 
 
 inline_for_extraction noextract
-val point_mul_double_split_lambda_vartime_noalloc:
+val point_mul_g_double_split_lambda_vartime_noalloc:
     out:point
   -> r1:qelem -> q1:point
   -> r2:qelem -> q2:point
@@ -580,7 +423,7 @@ val point_mul_double_split_lambda_vartime_noalloc:
 
     disjoint q4 scalar1 /\ disjoint q4 scalar2 /\ disjoint q4 p1 /\ disjoint q4 p2 /\
 
-    point_inv h p1 /\ point_inv h p2 /\
+    point_inv h p1 /\ point_inv h p2 /\ point_eval h p1 == S.g /\
     qas_nat h scalar1 < S.q /\ qas_nat h scalar2 < S.q)
   (ensures  fun h0 _ h1 -> modifies (loc r1 |+| loc r2 |+| loc r3 |+| loc r4 |+|
     loc q1 |+| loc q2 |+| loc q3 |+| loc q4 |+| loc out) h0 h1 /\
@@ -590,12 +433,13 @@ val point_mul_double_split_lambda_vartime_noalloc:
       (S.aff_point_mul (qas_nat h0 scalar1) (S.to_aff_point (point_eval h0 p1)))
       (S.aff_point_mul (qas_nat h0 scalar2) (S.to_aff_point (point_eval h0 p2))))
 
-let point_mul_double_split_lambda_vartime_noalloc out r1 q1 r2 q2 r3 q3 r4 q4
+let point_mul_g_double_split_lambda_vartime_noalloc out r1 q1 r2 q2 r3 q3 r4 q4
   scalar1 scalar2 p1 p2 =
   let h0 = ST.get () in
   let is_high1, is_high2, is_high3, is_high4 =
-   point_mul_double_split_lambda_vartime_noalloc_12 r1 q1 r2 q2 r3 q3 r4 q4 scalar1 scalar2 p1 p2 in
-  point_mul_double_split_lambda_table out r1 q1 r2 q2 r3 q3 r4 q4
+   point_mul_g_double_split_lambda_vartime_endo_split
+     r1 q1 r2 q2 r3 q3 r4 q4 scalar1 scalar2 p1 p2 in
+  point_mul_g_double_split_lambda_table out r1 q1 r2 q2 r3 q3 r4 q4
     p1 p2 is_high1 is_high2 is_high3 is_high4;
   let h1 = ST.get () in
   assert (S.to_aff_point (point_eval h1 out) ==
@@ -608,7 +452,7 @@ let point_mul_double_split_lambda_vartime_noalloc out r1 q1 r2 q2 r3 q3 r4 q4
 
 
 inline_for_extraction noextract
-val point_mul_double_split_lambda_vartime_noalloc_aux:
+val point_mul_g_double_split_lambda_vartime_noalloc_aux:
     out:point
   -> r1234:lbuffer uint64 16ul
   -> q1234:lbuffer uint64 60ul
@@ -627,7 +471,7 @@ val point_mul_double_split_lambda_vartime_noalloc_aux:
 
     disjoint q1234 scalar1 /\ disjoint q1234 scalar2 /\ disjoint q1234 p1 /\ disjoint q1234 p2 /\
 
-    point_inv h p1 /\ point_inv h p2 /\
+    point_inv h p1 /\ point_inv h p2 /\ point_eval h p1 == S.g /\
     qas_nat h scalar1 < S.q /\ qas_nat h scalar2 < S.q)
   (ensures  fun h0 _ h1 -> modifies (loc r1234 |+| loc q1234 |+| loc out) h0 h1 /\
     point_inv h1 out /\
@@ -636,7 +480,7 @@ val point_mul_double_split_lambda_vartime_noalloc_aux:
       (S.aff_point_mul (qas_nat h0 scalar1) (S.to_aff_point (point_eval h0 p1)))
       (S.aff_point_mul (qas_nat h0 scalar2) (S.to_aff_point (point_eval h0 p2))))
 
-let point_mul_double_split_lambda_vartime_noalloc_aux out r1234 q1234 scalar1 scalar2 p1 p2 =
+let point_mul_g_double_split_lambda_vartime_noalloc_aux out r1234 q1234 scalar1 scalar2 p1 p2 =
   let r1 = sub r1234 0ul 4ul in
   let r2 = sub r1234 4ul 4ul in
   let r3 = sub r1234 8ul 4ul in
@@ -646,16 +490,18 @@ let point_mul_double_split_lambda_vartime_noalloc_aux out r1234 q1234 scalar1 sc
   let q2 = sub q1234 15ul 15ul in
   let q3 = sub q1234 30ul 15ul in
   let q4 = sub q1234 45ul 15ul in
-  point_mul_double_split_lambda_vartime_noalloc out r1 q1 r2 q2 r3 q3 r4 q4 scalar1 scalar2 p1 p2
+  point_mul_g_double_split_lambda_vartime_noalloc
+    out r1 q1 r2 q2 r3 q3 r4 q4 scalar1 scalar2 p1 p2
 
 
-val point_mul_double_split_lambda_vartime:
+inline_for_extraction noextract
+val point_mul_g_double_split_lambda_vartime_alloc:
   out:point -> scalar1:qelem -> p1:point -> scalar2:qelem -> p2:point -> Stack unit
   (requires fun h ->
     live h out /\ live h scalar1 /\ live h p1 /\ live h scalar2 /\ live h p2 /\
     disjoint p1 out /\ disjoint p2 out /\ eq_or_disjoint p1 p2 /\
     disjoint scalar1 out /\ disjoint scalar2 out /\
-    point_inv h p1 /\ point_inv h p2 /\
+    point_inv h p1 /\ point_inv h p2 /\ point_eval h p1 == S.g /\
     qas_nat h scalar1 < S.q /\ qas_nat h scalar2 < S.q)
   (ensures fun h0 _ h1 -> modifies (loc out) h0 h1 /\
     point_inv h1 out /\
@@ -664,27 +510,13 @@ val point_mul_double_split_lambda_vartime:
       (S.aff_point_mul (qas_nat h0 scalar1) (S.to_aff_point (point_eval h0 p1)))
       (S.aff_point_mul (qas_nat h0 scalar2) (S.to_aff_point (point_eval h0 p2))))
 
-[@CInline]
-let point_mul_double_split_lambda_vartime out scalar1 p1 scalar2 p2 =
+let point_mul_g_double_split_lambda_vartime_alloc out scalar1 p1 scalar2 p2 =
   push_frame ();
   let r1234 = create 16ul (u64 0) in
   let q1234 = create 60ul (u64 0) in
-  point_mul_double_split_lambda_vartime_noalloc_aux out r1234 q1234 scalar1 scalar2 p1 p2;
+  point_mul_g_double_split_lambda_vartime_noalloc_aux out r1234 q1234 scalar1 scalar2 p1 p2;
   pop_frame ()
 
-
-val point_mul_g_double_split_lambda_vartime:
-  out:point -> scalar1:qelem -> scalar2:qelem -> p2:point ->
-  Stack unit
-  (requires fun h ->
-    live h out /\ live h scalar1 /\ live h scalar2 /\ live h p2 /\
-    disjoint p2 out /\ disjoint out scalar1 /\ disjoint out scalar2 /\
-    point_inv h p2 /\ qas_nat h scalar1 < S.q /\ qas_nat h scalar2 < S.q)
-  (ensures fun h0 _ h1 -> modifies (loc out) h0 h1 /\
-    point_inv h1 out /\
-    S.to_aff_point (point_eval h1 out) ==
-    S.to_aff_point (S.point_mul_double_g
-      (qas_nat h0 scalar1) (qas_nat h0 scalar2) (point_eval h0 p2)))
 
 [@CInline]
 let point_mul_g_double_split_lambda_vartime out scalar1 scalar2 p2 =
@@ -697,5 +529,5 @@ let point_mul_g_double_split_lambda_vartime out scalar1 scalar2 p2 =
   push_frame ();
   let g = create 15ul (u64 0) in
   make_g g;
-  point_mul_double_split_lambda_vartime out scalar1 g scalar2 p2;
+  point_mul_g_double_split_lambda_vartime_alloc out scalar1 g scalar2 p2;
   pop_frame ()
